env/stat.ml
@@ -1,0 +1,71 @@
+type stat = {
+  is_rec : bool;
+  code_size : int;
+  code_branchs : int;
+  code_effects : int;
+  code_lits : int;
+  smt_query_time_record : float list;
+  inclusion_query_time_record : float list;
+  max_inclusion_alphabet : int;
+  max_inclusion_automaton_size : int;
+}
+
+let init (is_rec, code_size, code_branchs, code_effects) =
+  {
+    is_rec;
+    code_size;
+    code_branchs;
+    code_effects;
+    code_lits = 0;
+    smt_query_time_record = [];
+    inclusion_query_time_record = [];
+    max_inclusion_alphabet = 0;
+    max_inclusion_automaton_size = 0;
+  }
+
+let update_dynamic_stat stat
+    ( smt_query_time_record,
+      inclusion_query_time_record,
+      max_inclusion_alphabet,
+      max_inclusion_automaton_size ) code_lits =
+  {
+    stat with
+    code_lits;
+    smt_query_time_record;
+    inclusion_query_time_record;
+    max_inclusion_alphabet;
+    max_inclusion_automaton_size;
+  }
+
+let dump_one stat =
+  `Assoc
+    [
+      ("is_rec", `Bool stat.is_rec);
+      ("code_size", `Int stat.code_size);
+      ("code_branchs", `Int stat.code_branchs);
+      ("code_effects", `Int stat.code_effects);
+      ("code_lits", `Int stat.code_lits);
+      ( "smt_query_time_record",
+        `List (List.map (fun x -> `Float x) stat.smt_query_time_record) );
+      ( "inclusion_query_time_record",
+        `List (List.map (fun x -> `Float x) stat.inclusion_query_time_record) );
+      ("max_inclusion_alphabet", `Int stat.max_inclusion_alphabet);
+      ("max_inclusion_automaton_size", `Int stat.max_inclusion_automaton_size);
+    ]
+
+let dump filename stats =
+  let j =
+    `List
+      (List.map
+         (fun (idx, if_well_typed, stat) ->
+           `Assoc
+             [
+               ("idx", `Int idx);
+               ("stat", dump_one stat);
+               ("if_well_typed", `Bool if_well_typed);
+             ])
+         stats)
+  in
+  let oc = Core.Out_channel.create filename in
+  Yojson.Basic.to_channel oc j;
+  Core.Out_channel.close oc
