regquery/check.ml
@@ -46,7 +46,10 @@ let smt_neg_and_solve ctx pre vc =
   (* let _ = printf "check\n" in *)
   let solver = mk_solver ctx None in
   let g = mk_goal ctx true false false in
-  let () = Printf.printf "Q: %s\n" @@ Language.Rty.layout_prop vc in
+  let () =
+    Env.show_debug_query @@ fun _ ->
+    Printf.printf "Q: %s\n" @@ Language.Rty.layout_prop vc
+  in
   (* let () = Printf.printf "Q: %s\n" @@ Frontend.coq_layout vc in *)
   (* let () = failwith "zz" in *)
   let time_t, q =
