scripts/analyze.py
@@ -1,0 +1,26 @@
+import sys
+import argparse
+import os
+import subprocess
+
+import statistics
+
+def num_total_avg (l):
+    return (len(l),
+            "{:.2f}".format(sum(l)),
+            "{:.2f}".format(statistics.mean(l)))
+
+def analyze (stat):
+    if len(stat) != 1:
+        print("each benchmark should has one function implementation")
+        exit(1)
+    stat = stat[0]["stat"]
+    num_smt, time_smt, time_smt_avg = num_total_avg(stat["smt_query_time_record"])
+    num_reg, time_reg, time_reg_avg = num_total_avg(stat["inclusion_query_time_record"])
+    stat["num_smt"] = num_smt
+    stat["time_smt"] = time_smt
+    stat["time_smt_avg"] = time_smt_avg
+    stat["num_reg"] = num_reg
+    stat["time_reg"] = time_reg
+    stat["time_reg_avg"] = time_reg_avg
+    return stat
