scripts/benchs.py
@@ -1,0 +1,25 @@
+import sys
+import argparse
+import os
+import json
+
+meta_config_file = "meta-config.json"
+
+def load (tab):
+    top_dir = tab['benchmark_dir']
+    res = {}
+    for info in tab['benchmarks_info']:
+        source = info["benchmark_source"]
+        for entry in info['benchmarks']:
+            path = "{}/{}".format(top_dir,entry.lower())
+            res[entry] = (source, path)
+    return res
+
+def load_benchmarks ():
+    with open (meta_config_file) as f:
+        j = json.load(f)
+        resfile = j['resfile']
+        benchmark_table_file = j['benchmark_table_file']
+        with open (benchmark_table_file) as f:
+            benchmark_table = json.load(f)
+    return load(benchmark_table)
