scripts/comprehensive.py
@@ -1,0 +1,37 @@
+import sys
+import argparse
+import os
+import subprocess
+import colored
+import benchs
+import run
+import analyze
+import mk_table
+import json
+
+meta_config_file = "meta-config.json"
+stat_file = ".stat.json"
+
+def run_all_benchs(verbose):
+    tab = benchs.load_benchmarks()
+    res = {}
+    for name, (source, path) in tab.items():
+        run.typecheck(path, verbose)
+        with open (stat_file) as f:
+            j = json.load(f)
+            stat = analyze.analyze(j)
+            stat["source"] = source
+            res[name] = analyze.analyze(j)
+            # break
+    mk_table.show_latex_tab(res)
+    return
+
+if __name__ == '__main__':
+    try:
+        if sys.argv[2] == "verbose":
+            verbose = True
+    except:
+        verbose = False
+    if "table1" == sys.argv[1]:
+        run_all_benchs(verbose)
+
