scripts/mk_table.py
@@ -1,0 +1,62 @@
+import sys
+import argparse
+import os
+import json
+from tabulate import tabulate
+
+headers = ["", "Recursive", "#LocalVar" , "#OP" , "#Q_{SMT}" , "#Q_{automata}" , "(max. Char, Size)" ,
+           "smt total (avg. time)(s)", "automata total (avg. time)(s)"]
+
+latex_headers = ["", "(\\#LocalVar, \\#Lit)" , "\\#OP" , "\\#Q$_{SMT}$" , "\\#Q$_{A}$" , "max. size$_{A}$" ,
+           "t$_{SMT}$ total (avg.)(s)", "t$_{A}$ total (avg.)(s)"]
+
+def show_source(source, name):
+    tab = {"Protocols": "⬦", "Algebraic Effects": "*",  "Datatypes": "◯", "leonidas": "★", "stlc": ""}
+    return "{} {}".format(name, tab[source])
+
+def show_is_rec(is_rec, branches):
+    if is_rec:
+        return [branches, "✓"]
+    else:
+        return [branches, ""]
+
+def show_is_rec_latex(is_rec):
+    if is_rec:
+        return "$\\checkmark$"
+    else:
+        return ""
+
+def show_data(data):
+    print("\n")
+    lines = []
+    for (source, is_rec, res) in data:
+        res = [show_source(source, res[0])] + show_is_rec(is_rec, res[1]) + res[2:]
+        lines.append(res)
+    print(tabulate(lines, headers, tablefmt='orgtbl', numalign="left"))
+
+def latex_name(name):
+    name = name.replace("_", "\_")
+    name = "\\textsf{" + name + "}"
+    # print(name)
+    return name
+
+def show_latex_tab(data):
+    print("\n")
+    header_str = " & ".join(latex_headers)
+    print("""
+\\toprule
+ {}\\\\
+\\midrule""".format(header_str))
+    for name, stat in data.items():
+        line = "{} & $({}, {})$ & ${}$ & ${}$ & ${}$ & ${}$ & $({},{})$ & $({},{})$ \\\\".format(
+            latex_name(name),
+            # show_is_rec_latex(stat["is_rec"]),
+            stat["code_size"],stat["code_lits"],
+            stat["code_effects"], stat["num_smt"], stat["num_reg"],
+            # stat["max_inclusion_alphabet"],
+            stat["max_inclusion_automaton_size"],
+            stat["time_smt"], stat["time_smt_avg"],
+            stat["time_reg"], stat["time_reg_avg"]
+        )
+        print(line)
+    print("\\bottomrule")
