typecheck/typecheck.ml
@@ -11,6 +11,7 @@ let check opctx' structure normalized_structure =
   (*   Printf.printf "Structure:\n%s\n" @@ Structure.layout_structure structure *)
   (* in *)
   let opctx, rctx = POpCtx.from_code structure in
+  let num_effects = List.length opctx in
   let opctx = opctx @ opctx' in
   (* let eqctx = Eqctx.from_code structure in *)
   (* let () = Printf.printf "!!! %s\n" @@ Eqctx.layout_equations eqctx in *)
@@ -30,7 +31,7 @@ let check opctx' structure normalized_structure =
         with
         | None -> _failatwith __FILE__ __LINE__ ""
         | Some (_, comp) ->
-            let () = Printf.printf "%s\n" @@ Nt.layout comp.P.ty in
+            (* let () = Printf.printf "%s\n" @@ Nt.layout comp.P.ty in *)
             let () =
               if not (Nt.eq comp.P.ty (R.erase rty)) then
                 let () =
@@ -46,7 +47,16 @@ let check opctx' structure normalized_structure =
               else ()
             in
             (* let () = failwith "end" in *)
+            let num_branchs = TypedCoreEff.stat_count_comp_branchs comp in
+            let num_vars = TypedCoreEff.stat_count_comp_vars comp in
+            let is_rec = TypedCoreEff.stat_is_rec comp in
+            let stat = Stat.init (is_rec, num_vars, num_branchs, num_effects) in
+            let () = Smtquery.stat_init () in
             let res = Bidirectional.comp_type_check { rctx; opctx } comp rty in
+            let num_lits = Desymbolic.get_max_lits () in
+            let stat =
+              Stat.update_dynamic_stat stat (Smtquery.stat_get_cur ()) num_lits
+            in
             let () =
               if res then
                 Env.show_debug_typing @@ fun _ ->
@@ -56,7 +66,7 @@ let check opctx' structure normalized_structure =
                 Env.show_debug_typing @@ fun _ ->
                 Pp.printf "@{<bold>@{<red>Task %i, type check failed@}@}\n" id
             in
-            (id, res))
+            (id, res, stat))
       tasks
   in
   ress
